
\documentclass[a4paper,12pt]{article}

%%%%%%%%%%%%%%%%%%%%%%%%%%%%%%%%%%%%%%%%%%%%%%%%%%%%%%%%%%%%%%%%%%%%%%%%%%%%%%%%%%%%%%%%%%%%%%%%%%%%%%%%%%%%%%%%%%%%%%%%%%%%%%%%%%%%%%%%%%%%%%%%%%%%%%%%%%%%%%%%%%%%%%%%%%%%%%%%%%%%%%%%%%%%%%%%%%%%%%%%%%%%%%%%%%%%%%%%%%%%%%%%%%%%%%%%%%%%%%%%%%%%%%%%%%%%
  \usepackage{eurosym}
\usepackage{vmargin}
\usepackage{amsmath}
\usepackage{graphics}
\usepackage{epsfig}
\usepackage{enumerate}
\usepackage{multicol}
\usepackage{subfigure}
\usepackage{fancyhdr}
\usepackage{listings}
\usepackage{framed}
\usepackage{graphicx}
\usepackage{amsmath}
\usepackage{chngpage}
%\usepackage{bigints}
\usepackage{vmargin}

% left top textwidth textheight headheight

% headsep footheight footskip

\setmargins{2.0cm}{2.5cm}{16 cm}{22cm}{0.5cm}{0cm}{1cm}{1cm}

\renewcommand{\baselinestretch}{1.3}

\setcounter{MaxMatrixCols}{10}

\begin{document}

\begin{enumerate}
\item % Question 6
Consider two random variables X and Y with joint probability density function (pdf)
\[f ( x , y ) =
4
(1 − xy ) , 0 < x < 1, 0 < y < 1 .
3\]
The marginal pdf of X is given by
\[f ( x ) =
2
(2 − x ) , 0 < x < 1
3\]
with a corresponding marginal pdf for $Y$ by symmetry (you are not asked to verify these marginal densities).
\begin{enumerate}
    \item (i)
Show that the conditional pdf of Y given $X = x$ is given by
f ( y | x ) = 2
\item (ii)
(1 − xy )
, 0 < y < 1.
(2 − x )

(a) Determine the conditional expectation $E ( Y | X = x )$ as a function of $x$ and hence determine $E ( Y )$ .
(b) Verify your answer in part (a) by determining $E ( Y )$ directly from the marginal pdf of $Y$.
\end{enumerate}
\end{enumerate}

\newpage
\begin{framed}
If both X and Y are continuous random variables, then the conditional expectation is

\[{\displaystyle \operatorname {E} (X\mid Y=y)=\int _{\mathcal {X}}xf_{X\mid Y}(x\mid y)\,\mathrm {d} x,} \]

where $ {\displaystyle f_{X\mid Y}(x\mid y)={\frac {f_{X,Y}(x,y)}{f_{Y}(y)}}}$ 
(where fY(y) gives the density of Y). 
\end{framed}
%%%%%%%%%%%%%%%%%%%%%%%%%%%%%%%%%%%%%%%%%%%%%%%
%%- Question 6 Solution
(i)
\[ f(y|x) = \frac{f(x,y)}{f(x)}\]

\begin{eqnarray*}
 f(y|x) &=& \frac{f(x,y)}{f(x)}  \\
 &=& \frac{  \frac{4}{3} (1\;-\;xy) }{\frac{2}{3} (2\;-\;x)  }  \\
 &=& 2 \frac{(1\;-\;xy)}{(2\;-\;x)} \mbox{ 0 < y <1 }  \\
 \end{eqnarray*}
 
 
 %%%%%%%%%%%%%%%%%%%%%%%%%%%%%%%%%%
 
 \begin{eqnarray*}
 E(Y|X=x) &=& \frac{2}{(2-x)} \int^{}_{0} y(1-y) dy \\
  &=& \frac{2}{(2-x)} \left[  \frac{y^2}{2} - x \frac{y^3}{3}\right]^{1}_{0} \\ 
  &=& \frac{2}{(2-x)} \left[  \frac{1}{2} -  \frac{x}{3}\right] \\ 
  &=& \frac{2}{(2-x)} \left[  \frac{3}{6} -  \frac{2x}{6}\right] \\ 
  &=& \frac{3\;-\;2x}{3(2\;-\;x)}
 \end{eqnarray*}
 
 \begin{eqnarray*}
 E(Y) &=& \int^{1}{0} \frac{3\;-\;2x}{3(2\;-\;x)} \frac{2}{3} (2-x) dx
 &=& \frac{2}{9} \int^{1}{0}  (3 \;-\;2x) dx \\
 &=&  \frac{2}{9}  \left[  3x - x^2 \right]^{1}_{0} \\
&=&  \frac{2}{9}  \left[  3- 1 \right]^{1}_{0} \\ 
&=& \frac{4}{9}
\end{eqnarray*}
\end{document}

